lava/out/Benchmark/SoftwareFoundationsInduction.v
@@ -1,20 +1,24 @@
-
+From coqDeps Require Export LiquidPreludeUtil.
+Open Scope Z_scope.
+Open Scope Int_scope.
+Set Universe Polymorphism.
+From Coq Require Import Unicode.Utf8.
 
 Load Benchmark.SoftwareFoundationsBasics.
 
-Definition plus_n_Sm_spec (ds_d9ab m : MyNat): Type :=
+Definition plus_n_Sm_spec (ds_d9a8 m : MyNat): Type :=
   {{∃ (plus_res : MyNat_u),
-    plus_rel ⌊ ds_d9ab -⌋ ⌊ m -⌋ plus_res
+    plus_rel ⌊ ds_d9a8 -⌋ ⌊ m -⌋ plus_res
     ∧ ∃ (plus_res_2 : MyNat_u),
-      plus_rel ⌊ ds_d9ab -⌋ (S_u ⌊ m -⌋) plus_res_2 ∧ S_u plus_res == plus_res_2}}.
+      plus_rel ⌊ ds_d9a8 -⌋ (S_u ⌊ m -⌋) plus_res_2 ∧ S_u plus_res == plus_res_2}}.
 
 #[global] Hint Unfold plus_n_Sm_spec: lia_unfold.
 
-Theorem plus_n_Sm (ds_d9ab m : MyNat): plus_n_Sm_spec ds_d9ab m.
+Theorem plus_n_Sm (ds_d9a8 m : MyNat): plus_n_Sm_spec ds_d9a8 m.
 Proof.
-  destruct ds_d9ab as [ds_d9ab ds_d9ab_p].
+  destruct ds_d9a8 as [ds_d9a8 ds_d9a8_p].
   destruct m as [m m_p].
-  try revert m_p; generalize dependent m; induction ds_d9ab as [| n' IH_n']; intros.
+  try revert m_p; generalize dependent m; induction ds_d9a8 as [| n' IH_n']; intros.
   - refine (subsumptionCast
             Unit
             (λ (VV : Unit),
@@ -33,15 +37,15 @@ Proof.
             ltac:(solver)).
 Qed.
 
-Definition mul_0_r_spec (ds_d9ac : MyNat): Type :=
-  {{∃ (mult_res : MyNat_u), mult_rel ⌊ ds_d9ac -⌋ O_u mult_res ∧ mult_res == O_u}}.
+Definition mul_0_r_spec (ds_d9a9 : MyNat): Type :=
+  {{∃ (mult_res : MyNat_u), mult_rel ⌊ ds_d9a9 -⌋ O_u mult_res ∧ mult_res == O_u}}.
 
 #[global] Hint Unfold mul_0_r_spec: lia_unfold.
 
-Theorem mul_0_r (ds_d9ac : MyNat): mul_0_r_spec ds_d9ac.
+Theorem mul_0_r (ds_d9a9 : MyNat): mul_0_r_spec ds_d9a9.
 Proof.
-  destruct ds_d9ac as [ds_d9ac ds_d9ac_p].
-  induction ds_d9ac as [| n' IH_n'].
+  destruct ds_d9a9 as [ds_d9a9 ds_d9a9_p].
+  induction ds_d9a9 as [| n' IH_n'].
   - refine (subsumptionCast
             Unit
             (λ (VV : Unit), ∃ (mult_res : MyNat_u), mult_rel O_u O_u mult_res ∧ mult_res == O_u)
@@ -54,15 +58,15 @@ Proof.
             ltac:(solver)).
 Qed.
 
-Definition minus_n_n_spec (ds_d9ad : MyNat): Type :=
-  {{∃ (minus_res : MyNat_u), minus_rel ⌊ ds_d9ad -⌋ ⌊ ds_d9ad -⌋ minus_res ∧ minus_res == O_u}}.
+Definition minus_n_n_spec (ds_d9aa : MyNat): Type :=
+  {{∃ (minus_res : MyNat_u), minus_rel ⌊ ds_d9aa -⌋ ⌊ ds_d9aa -⌋ minus_res ∧ minus_res == O_u}}.
 
 #[global] Hint Unfold minus_n_n_spec: lia_unfold.
 
-Theorem minus_n_n (ds_d9ad : MyNat): minus_n_n_spec ds_d9ad.
+Theorem minus_n_n (ds_d9aa : MyNat): minus_n_n_spec ds_d9aa.
 Proof.
-  destruct ds_d9ad as [ds_d9ad ds_d9ad_p].
-  induction ds_d9ad as [| n' IH_n'].
+  destruct ds_d9aa as [ds_d9aa ds_d9aa_p].
+  induction ds_d9aa as [| n' IH_n'].
   - refine (subsumptionCast
             Unit
             (λ (VV : Unit), ∃ (minus_res : MyNat_u), minus_rel O_u O_u minus_res ∧ minus_res == O_u)
@@ -75,15 +79,15 @@ Proof.
             ltac:(solver)).
 Qed.
 
-Definition add_0_r_spec (ds_d9ae : MyNat): Type :=
-  {{∃ (plus_res : MyNat_u), plus_rel ⌊ ds_d9ae -⌋ O_u plus_res ∧ plus_res == ⌊ ds_d9ae -⌋}}.
+Definition add_0_r_spec (ds_d9ab : MyNat): Type :=
+  {{∃ (plus_res : MyNat_u), plus_rel ⌊ ds_d9ab -⌋ O_u plus_res ∧ plus_res == ⌊ ds_d9ab -⌋}}.
 
 #[global] Hint Unfold add_0_r_spec: lia_unfold.
 
-Theorem add_0_r (ds_d9ae : MyNat): add_0_r_spec ds_d9ae.
+Theorem add_0_r (ds_d9ab : MyNat): add_0_r_spec ds_d9ab.
 Proof.
-  destruct ds_d9ae as [ds_d9ae ds_d9ae_p].
-  induction ds_d9ae as [| n' IH_n'].
+  destruct ds_d9ab as [ds_d9ab ds_d9ab_p].
+  induction ds_d9ab as [| n' IH_n'].
   - refine (subsumptionCast
             Unit
             (λ (VV : Unit), ∃ (plus_res : MyNat_u), plus_rel O_u O_u plus_res ∧ plus_res == O_u)
@@ -96,18 +100,18 @@ Proof.
             ltac:(solver)).
 Qed.
 
-Definition add_comm_spec (ds_d9af m : MyNat): Type :=
+Definition add_comm_spec (ds_d9ac m : MyNat): Type :=
   {{∃ (plus_res : MyNat_u),
-    plus_rel ⌊ ds_d9af -⌋ ⌊ m -⌋ plus_res
-    ∧ ∃ (plus_res_2 : MyNat_u), plus_rel ⌊ m -⌋ ⌊ ds_d9af -⌋ plus_res_2 ∧ plus_res == plus_res_2}}.
+    plus_rel ⌊ ds_d9ac -⌋ ⌊ m -⌋ plus_res
+    ∧ ∃ (plus_res_2 : MyNat_u), plus_rel ⌊ m -⌋ ⌊ ds_d9ac -⌋ plus_res_2 ∧ plus_res == plus_res_2}}.
 
 #[global] Hint Unfold add_comm_spec: lia_unfold.
 
-Theorem add_comm (ds_d9af m : MyNat): add_comm_spec ds_d9af m.
+Theorem add_comm (ds_d9ac m : MyNat): add_comm_spec ds_d9ac m.
 Proof.
-  destruct ds_d9af as [ds_d9af ds_d9af_p].
+  destruct ds_d9ac as [ds_d9ac ds_d9ac_p].
   destruct m as [m m_p].
-  try revert m_p; generalize dependent m; induction ds_d9af as [| n' IH_n']; intros.
+  destruct ds_d9ac as [| n'].
   - refine (subsumptionCast
             Unit
             (λ (VV : Unit),
@@ -116,17 +120,17 @@ Proof.
              ∧ ∃ (plus_res_2 : MyNat_u), plus_rel m O_u plus_res_2 ∧ plus_res == plus_res_2)
             (add_0_r (exist (λ (m : MyNat_u), MyNat_wf m ∧ True) m ltac:(solver)))
             ltac:(solver)).
-  - refine (subsumptionCast
+  - assert (h_15156453 : plus n' m ==? plus m n').
+    { refine (add_comm
+              (exist (λ (VV : MyNat_u), MyNat_wf VV ∧ True) n' ltac:(solver))
+              (exist (λ (m : MyNat_u), MyNat_wf m ∧ True) m ltac:(solver))). }
+    refine (subsumptionCast
             Unit
             (λ (VV : Unit),
              ∃ (plus_res : MyNat_u),
              plus_rel (S_u n') m plus_res
              ∧ ∃ (plus_res_2 : MyNat_u), plus_rel m (S_u n') plus_res_2 ∧ plus_res == plus_res_2)
-            (let H_91091155: ∃ (plus_res : MyNat_u),
-                             plus_rel n' m plus_res
-                             ∧ ∃ (plus_res_2 : MyNat_u), plus_rel m n' plus_res_2 ∧ plus_res == plus_res_2 :=
-             ⌈ IH_n' ltac:(try clear IH_n'; solver) m ltac:(try clear IH_n'; solver) ⌉ in
-             plus_n_Sm
+            (plus_n_Sm
              (exist (λ (m : MyNat_u), MyNat_wf m ∧ True) m ltac:(solver))
              (exist (λ (VV : MyNat_u), MyNat_wf VV ∧ True) n' ltac:(solver)))
             ltac:(solver)).
